DynamoDbEncryption/runtimes/java/src/main/smithy-generated/software/amazon/cryptography/dbencryptionsdk/dynamodb/model/oneToFiveInput.java
@@ -1,0 +1,71 @@
+// Copyright Amazon.com Inc. or its affiliates. All Rights Reserved.
+// SPDX-License-Identifier: Apache-2.0
+// Do not modify this file. This file is machine generated, and any changes to it will be overwritten.
+package software.amazon.cryptography.dbencryptionsdk.dynamodb.model;
+
+public class oneToFiveInput {
+
+  private final int inputOne;
+
+  protected oneToFiveInput(BuilderImpl builder) {
+    this.inputOne = builder.inputOne();
+  }
+
+  public int inputOne() {
+    return this.inputOne;
+  }
+
+  public Builder toBuilder() {
+    return new BuilderImpl(this);
+  }
+
+  public static Builder builder() {
+    return new BuilderImpl();
+  }
+
+  public interface Builder {
+    Builder inputOne(int inputOne);
+
+    int inputOne();
+
+    oneToFiveInput build();
+  }
+
+  static class BuilderImpl implements Builder {
+
+    protected int inputOne;
+
+    private boolean _inputOneSet = false;
+
+    protected BuilderImpl() {}
+
+    protected BuilderImpl(oneToFiveInput model) {
+      this.inputOne = model.inputOne();
+      this._inputOneSet = true;
+    }
+
+    public Builder inputOne(int inputOne) {
+      this.inputOne = inputOne;
+      this._inputOneSet = true;
+      return this;
+    }
+
+    public int inputOne() {
+      return this.inputOne;
+    }
+
+    public oneToFiveInput build() {
+      if (this._inputOneSet && this.inputOne() < 1) {
+        throw new IllegalArgumentException(
+          "`inputOne` must be greater than or equal to 1"
+        );
+      }
+      if (this._inputOneSet && this.inputOne() > 5) {
+        throw new IllegalArgumentException(
+          "`inputOne` must be less than or equal to 5."
+        );
+      }
+      return new oneToFiveInput(this);
+    }
+  }
+}
