DynamoDbEncryption/runtimes/java/src/main/smithy-generated/software/amazon/cryptography/dbencryptionsdk/dynamodb/model/oneToFiveOutput.java
@@ -1,0 +1,71 @@
+// Copyright Amazon.com Inc. or its affiliates. All Rights Reserved.
+// SPDX-License-Identifier: Apache-2.0
+// Do not modify this file. This file is machine generated, and any changes to it will be overwritten.
+package software.amazon.cryptography.dbencryptionsdk.dynamodb.model;
+
+public class oneToFiveOutput {
+
+  private final int outputOne;
+
+  protected oneToFiveOutput(BuilderImpl builder) {
+    this.outputOne = builder.outputOne();
+  }
+
+  public int outputOne() {
+    return this.outputOne;
+  }
+
+  public Builder toBuilder() {
+    return new BuilderImpl(this);
+  }
+
+  public static Builder builder() {
+    return new BuilderImpl();
+  }
+
+  public interface Builder {
+    Builder outputOne(int outputOne);
+
+    int outputOne();
+
+    oneToFiveOutput build();
+  }
+
+  static class BuilderImpl implements Builder {
+
+    protected int outputOne;
+
+    private boolean _outputOneSet = false;
+
+    protected BuilderImpl() {}
+
+    protected BuilderImpl(oneToFiveOutput model) {
+      this.outputOne = model.outputOne();
+      this._outputOneSet = true;
+    }
+
+    public Builder outputOne(int outputOne) {
+      this.outputOne = outputOne;
+      this._outputOneSet = true;
+      return this;
+    }
+
+    public int outputOne() {
+      return this.outputOne;
+    }
+
+    public oneToFiveOutput build() {
+      if (this._outputOneSet && this.outputOne() < 1) {
+        throw new IllegalArgumentException(
+          "`outputOne` must be greater than or equal to 1"
+        );
+      }
+      if (this._outputOneSet && this.outputOne() > 5) {
+        throw new IllegalArgumentException(
+          "`outputOne` must be less than or equal to 5."
+        );
+      }
+      return new oneToFiveOutput(this);
+    }
+  }
+}
