DynamoDbEncryption/runtimes/net/Generated/DynamoDbEncryption/DynamoDbEncryption.cs
@@ -40,5 +40,12 @@ namespace AWS.Cryptography.DbEncryptionSDK.DynamoDb
       if (result.is_Failure) throw TypeConversion.FromDafny_CommonError(result.dtor_error);
       return TypeConversion.FromDafny_N3_aws__N12_cryptography__N15_dbEncryptionSdk__N8_dynamoDb__S36_GetEncryptedDataKeyDescriptionOutput(result.dtor_value);
     }
+    public AWS.Cryptography.DbEncryptionSDK.DynamoDb.oneToFiveOutput TestOneToFive(AWS.Cryptography.DbEncryptionSDK.DynamoDb.oneToFiveInput input)
+    {
+      software.amazon.cryptography.dbencryptionsdk.dynamodb.internaldafny.types._IoneToFiveInput internalInput = TypeConversion.ToDafny_N3_aws__N12_cryptography__N15_dbEncryptionSdk__N8_dynamoDb__S14_oneToFiveInput(input);
+      Wrappers_Compile._IResult<software.amazon.cryptography.dbencryptionsdk.dynamodb.internaldafny.types._IoneToFiveOutput, software.amazon.cryptography.dbencryptionsdk.dynamodb.internaldafny.types._IError> result = _impl.TestOneToFive(internalInput);
+      if (result.is_Failure) throw TypeConversion.FromDafny_CommonError(result.dtor_error);
+      return TypeConversion.FromDafny_N3_aws__N12_cryptography__N15_dbEncryptionSdk__N8_dynamoDb__S15_oneToFiveOutput(result.dtor_value);
+    }
   }
 }
