DynamoDbEncryption/runtimes/net/Generated/DynamoDbEncryption/oneToFiveInput.cs
@@ -1,0 +1,37 @@
+// Copyright Amazon.com Inc. or its affiliates. All Rights Reserved.
+// SPDX-License-Identifier: Apache-2.0
+// Do not modify this file. This file is machine generated, and any changes to it will be overwritten.
+using System;
+using AWS.Cryptography.DbEncryptionSDK.DynamoDb;
+namespace AWS.Cryptography.DbEncryptionSDK.DynamoDb
+{
+  public class oneToFiveInput
+  {
+    private int? _inputOne;
+    public int InputOne
+    {
+      get { return this._inputOne.GetValueOrDefault(); }
+      set { this._inputOne = value; }
+    }
+    public bool IsSetInputOne()
+    {
+      return this._inputOne.HasValue;
+    }
+    public void Validate()
+    {
+      if (IsSetInputOne())
+      {
+        if (InputOne < 1)
+        {
+          throw new System.ArgumentException(
+              String.Format("Member InputOne of structure oneToFiveInput has type oneToFiveIp which has a minimum of 1 but was given the value {0}.", InputOne));
+        }
+        if (InputOne > 5)
+        {
+          throw new System.ArgumentException(
+              String.Format("Member InputOne of structure oneToFiveInput has type oneToFiveIp which has a maximum of 5 but was given the value {0}.", InputOne));
+        }
+      }
+    }
+  }
+}
