DynamoDbEncryption/runtimes/net/Generated/DynamoDbEncryption/oneToFiveOutput.cs
@@ -1,0 +1,37 @@
+// Copyright Amazon.com Inc. or its affiliates. All Rights Reserved.
+// SPDX-License-Identifier: Apache-2.0
+// Do not modify this file. This file is machine generated, and any changes to it will be overwritten.
+using System;
+using AWS.Cryptography.DbEncryptionSDK.DynamoDb;
+namespace AWS.Cryptography.DbEncryptionSDK.DynamoDb
+{
+  public class oneToFiveOutput
+  {
+    private int? _outputOne;
+    public int OutputOne
+    {
+      get { return this._outputOne.GetValueOrDefault(); }
+      set { this._outputOne = value; }
+    }
+    public bool IsSetOutputOne()
+    {
+      return this._outputOne.HasValue;
+    }
+    public void Validate()
+    {
+      if (IsSetOutputOne())
+      {
+        if (OutputOne < 1)
+        {
+          throw new System.ArgumentException(
+              String.Format("Member OutputOne of structure oneToFiveOutput has type oneToFiveOp which has a minimum of 1 but was given the value {0}.", OutputOne));
+        }
+        if (OutputOne > 5)
+        {
+          throw new System.ArgumentException(
+              String.Format("Member OutputOne of structure oneToFiveOutput has type oneToFiveOp which has a maximum of 5 but was given the value {0}.", OutputOne));
+        }
+      }
+    }
+  }
+}
